rt proof: update for merge breakages
Signed-off-by: Gerwin Klein <gerwin.klein@proofcraft.systems>

proof/refine/RISCV64/Detype_R.thy
@@ -100,8 +100,8 @@ defs deletionIsSafe_def:
         \<and> (\<forall>ko. ksPSpace s p = Some (KOArch ko) \<and> p \<in> {ptr .. ptr + 2 ^ bits - 1}
                 \<longrightarrow> 6 \<le> bits)"
 
-defs deletionIsSafe_delete_locale_def:
-  "deletionIsSafe_delete_locale \<equiv> \<lambda>ptr bits s. \<forall>p. ko_wp_at' live' p s \<longrightarrow> p \<notin> mask_range ptr bits"
+defs deletionIsSafe_delete_locale_def: (* FIXME merge: remove completely? *)
+  "deletionIsSafe_delete_locale \<equiv> \<lambda>ptr bits s. True"
 
 defs ksASIDMapSafe_def:
   "ksASIDMapSafe \<equiv> \<lambda>s. True"
@@ -479,7 +479,22 @@ lemma zobj_refs_capRange:
   "capAligned c \<Longrightarrow> zobj_refs' c \<subseteq> capRange c"
   by (cases c, simp_all add: capRange_def capAligned_def is_aligned_no_overflow)
 
-context delete_locale begin interpretation Arch . (*FIXME: arch_split*)
+end
+
+locale delete_locale =
+  fixes s' and base and bits and ptr and idx and d
+  assumes     cap: "cte_wp_at' (\<lambda>cte. cteCap cte = UntypedCap d base bits idx) ptr s'"
+  and      nodesc: "descendants_range' (UntypedCap d base bits idx) ptr (ctes_of s')"
+  and        invs: "invs' s'"
+  and    sym_refs: "sym_refs (state_refs_of' s')"
+  and valid_idle': "valid_idle' s'"
+  and      ct_act: "ct_active' s'"
+  and     sa_simp: "sch_act_simple s'"
+  and          al: "is_aligned base bits"
+  and      rlqrun: "\<forall>p. p \<in> set (ksReleaseQueue s') \<longrightarrow> obj_at' (runnable' \<circ> tcbState) p s'"
+begin
+
+interpretation Arch . (*FIXME: arch_split*)
 
 lemma  valid_objs: "valid_objs' s'"
   and    vreplies: "valid_replies' s'"
@@ -858,6 +873,7 @@ lemma deleteObjects_corres:
    apply (rule delete_locale.deletionIsSafe_holds;
           (fastforce simp: delete_locale_def valid_cap_simps sch_act_simple_def state_relation_def
                            sched_act_relation_def pred_conj_def)?)
+  apply (simp add: deletionIsSafe_delete_locale_def) (* FIXME merge: remove? *)
   apply (simp add: bind_assoc[symmetric])
   apply (rule corres_stateAssert_implied2)
      defer
@@ -3053,8 +3069,6 @@ lemma curDomain_commute:
   apply auto
   done
 
-crunch inv[wp]: curDomain P
-
 lemma placeNewObject_tcb_at':
   "\<lbrace>pspace_aligned' and pspace_distinct' and pspace_no_overlap' ptr (objBits (makeObject::tcb))
     and K(is_aligned ptr  (objBits (makeObject::tcb)))\<rbrace>
@@ -3062,8 +3076,17 @@ lemma placeNewObject_tcb_at':
    \<lbrace>\<lambda>_ s. tcb_at' ptr s \<rbrace>"
   apply (simp add:placeNewObject_def placeNewObject'_def split_def alignError_def)
   apply wpsimp
-  apply (clarsimp simp: obj_at'_def objBits_simps ps_clear_def)
-  apply (fastforce intro!: set_eqI dest: pspace_no_overlap_disjoint' simp: add_mask_fold)
+  apply (clarsimp simp: obj_at'_def lookupAround2_None1 objBits_simps
+                        lookupAround2_char1 field_simps projectKO_opt_tcb return_def ps_clear_def
+                  simp flip: is_aligned_mask)
+  apply (drule (1) pspace_no_overlap_disjoint')
+  apply (intro conjI impI allI)
+     apply (clarsimp intro!: set_eqI)
+     apply (metis add_mask_fold if_Some_Some)
+    apply (clarsimp simp: objBits_simps' word_bits_def)
+   apply (clarsimp intro!: set_eqI)
+   apply (simp add: add_mask_fold not_in_domD orthD1)
+  apply (clarsimp simp: objBits_simps' word_bits_def)
   done
 
 lemma monad_commute_if_weak_r:
